solvers/59.lean
@@ -1,4 +1,5 @@
 import Std
+import ProjectEulerStatements.P59
 namespace ProjectEulerSolutions.P59
 
 def parseNat (s : String) : Nat :=
@@ -84,6 +85,9 @@ example : Nat.xor 107 42 = 65 := by
 
 def solve (cipher : List Nat) : Nat :=
   bestKeyAndSum cipher
+
+theorem equiv (cipher : List Nat) :
+    ProjectEulerStatements.P59.naive cipher = solve cipher := sorry
 
 end ProjectEulerSolutions.P59
 open ProjectEulerSolutions.P59
